theories/Staging/UnifLogic.v
@@ -78,10 +78,6 @@ Module Pred
       fun t2 w t1 ι => (inst t1 ι = t2)%type.
     #[global] Arguments repₚ {T A _} _ [w] _ _/.
     
-    Definition proprepₚ {T : LCtx -> Type} {instTA : InstProp T} : Prop -> ⊢ Tm T -> Pred :=
-      fun t2 w t1 ι => (instprop t1 ι <-> t2)%type.
-    #[global] Arguments proprepₚ {T _} _ [w] _ _/.
-
   End Definitions.
   
   Section EntailmentDefinitions.
@@ -124,9 +120,9 @@ Module Pred
 
     #[export] Instance entails_rewriterelation : RewriteRelation (@entails w) := {}.
 
-    #[export] Instance proper_bientails :
-      Proper (@bientails w ==> @bientails w ==> iff) bientails.
-    Proof. crushPredEntails1. Qed.
+    (* #[export] Instance proper_bientails : *)
+    (*   Proper (@bientails w ==> @bientails w ==> iff) bientails. *)
+    (* Proof. crushPredEntails1. Qed. *)
     (* #[export] Instance proper_entails_bientails : *)
     (*   Proper ((≡@{Pred w}) ==> (≡@{Pred w}) ==> iff) entails. *)
     (* Proof. crushPredEntails1. Qed. *)
@@ -143,12 +139,12 @@ Module Pred
     Import iris.bi.interface.
     Import iris.bi.extensions.
 
-    Variant empₚ {w} (ι : Valuation w) : Prop :=
-      MkEmp : empₚ ι.
-    Variant sepₚ {w} (P Q : Pred w) (ι : Valuation w) : Prop :=
-      MkSep : P ι -> Q ι -> sepₚ P Q ι.
-    Variant wandₚ {w} (P Q : Pred w) (ι : Valuation w) : Prop :=
-      MkWand : (P ι -> Q ι) -> wandₚ P Q ι.
+    Definition empₚ {w} (ι : Valuation w) : Prop := True.
+    Arguments empₚ {w} ι /.
+    Definition sepₚ {w} (P Q : Pred w) (ι : Valuation w) : Prop := P ι /\ Q ι.
+    Arguments sepₚ {w} P Q ι /.
+    Definition wandₚ {w} (P Q : Pred w) (ι : Valuation w) : Prop := P ι -> Q ι.
+    Arguments wandₚ {w} P Q ι /.
     Variant persistently {w} (P : Pred w) (ι : Valuation w) : Prop :=
       MkSubstly : P ι -> persistently P ι.
 
@@ -184,7 +180,6 @@ Module Pred
         | [ |- equiv _ _] => constructor
         | [ H : ?H |- ?H ] => assumption
         | [ H1 : ?P1 -> ?P2, H2: ?P1  |- ?P2 ] => apply (H1 H2)
-        | [ H : ?H1 -> ?H2 |- ?H2 ] => apply H
         | [ H : ?H1 <-> ?H2 |- ?H2 ] => apply (proj1 H); clear H
         | [ H : ?H1 <-> ?H2 |- ?H1 ] => apply (proj2 H); clear H
         | [ H : ?P1 <-> ?P2, H2 : ?P1 |- _ ] => apply (proj1 H) in H2; clear H
@@ -200,8 +195,8 @@ Module Pred
         | [ |- sepₚ _ _ _ ] => split
         | [ |- eqₚ ?t1 ?t2 ?ι ] => intro
         (* | [ |- ∀ₚ _ ] => intro *)
-        | [ |- wandₚ _ _ _ ] => constructor; intros
-        | [ H : wandₚ _ _ _ |- _ ] => destruct H; cbn in H
+        | [ |- wandₚ _ _ _ ] => intro
+        | [ H : wandₚ _ _ _ |- _ ] => cbn in H
         | [ H : (fun x => _) _ |- _ ] => cbn in H
         | [ |- True ] => trivial
         | [ |- empₚ _ ] => constructor
@@ -230,11 +225,15 @@ Module Pred
           bi_persistently := persistently;
           bi_later := later;
         |}.
-      constructor; crushPredEntails2.
-      constructor; crushPredEntails2.
-      constructor; crushPredEntails2.
-
+      - constructor; crushPredEntails2.
+        apply H1; crushPredEntails2.
+      - constructor; crushPredEntails2.
+      - constructor; crushPredEntails2.
     Defined.
+
+    Definition proprepₚ {T : LCtx -> Type} {instTA : InstProp T} : Prop -> forall w, Tm T w -> Pred w :=
+      fun t2 w t1 => ((instprop t1 : Pred w) ∗-∗ bi_pure t2)%I.
+    #[global] Arguments proprepₚ {T _} _ [w] _ _/.
 
     #[export] Instance persistent_pred {w} {P : Pred w} :
       derived_connectives.Persistent P.
@@ -247,6 +246,7 @@ Module Pred
 
     #[export] Instance pred_pure_forall {w} : BiPureForall (Pred w).
     Proof. constructor. crushPredEntails2. Qed.
+
   End proofmode.
 
   Ltac punfold_connectives :=
@@ -254,11 +254,10 @@ Module Pred
     change (@interface.bi_sep (@bi_pred ?w) ?P ?Q ?ι) with (sepₚ (w := w) P Q ι) in * ||
     change (@eqₚ ?T ?A ?instTA ?w ?t1 ?t2 ?ι) with (inst t1 ι = inst t2 ι) in * ||
     change (@repₚ ?T ?A ?instTA ?t2 ?w ?t1 ?ι) with (inst t1 ι = t2) in *||
-    change (@eqₚ ?T ?A ?instTA ?w ?t1 ?t2 ?ι) with (inst t1 ι = inst t2 ι) in * ||
-    change (@repₚ ?T ?A ?instTA ?t2 ?w ?t1 ?ι) with (inst t1 ι = t2) in *||
+    change (@wandₚ ?w ?P ?Q ?ι) with (P ι -> Q ι) in *||
     change (@proprepₚ ?T ?instTP ?t2 ?w ?t1 ?ι) with (instprop t1 ι <-> t2) in *||
     change (@interface.bi_emp (@bi_pred _) ?ι) with (empₚ ι) in *||
-    change (@interface.bi_wand (@bi_pred _) ?P ?Q ?ι) with (wandₚ P Q ι) in *||
+    change (@interface.bi_wand (@bi_pred ?w) ?P ?Q ?ι) with (@wandₚ w P Q ι) in *||
     change (@interface.bi_entails (@bi_pred _) ?P ?Q) with (entails P Q) in *||
     change (@interface.bi_persistently (@bi_pred _) ?P ?ι) with (persistently P ι) in *||
     change (@interface.bi_or (@bi_pred ?w) ?P ?Q ?ι) with (P ι \/ Q ι) in *||
@@ -268,7 +267,7 @@ Module Pred
     change (@interface.bi_forall (@bi_pred ?w) ?A ?f ?ι) with (forall a, f a ι) ||
     (* the change seems to trigger some coq binding bug, so I removed the "in *" for now... *)
     change (@interface.bi_exist (@bi_pred ?w) ?A ?P) with (fun ι => exists a : A, P a ι) in *||
-    unfold derived_connectives.bi_intuitionistically, derived_connectives.bi_affinely, interface.bi_emp_valid in *;
+    unfold derived_connectives.bi_wand_iff, derived_connectives.bi_intuitionistically, derived_connectives.bi_affinely, interface.bi_emp_valid, proprepₚ in *;
     (* change (@subst Pred subst_pred _ _ ?P _ ?θ ?ι) with (P (inst θ ι)) in *; *)
     try progress (cbn beta).
   (* Ltac crushPredEntailsMatch3 := *)
@@ -323,6 +322,12 @@ Module Pred
 
   End notations.
 
+  #[export] Instance pred_absorbing {w} {P : Pred w} : derived_connectives.Absorbing P.
+  Proof.
+    unfold derived_connectives.Absorbing, derived_connectives.bi_absorbingly.
+    crushPredEntails3.
+  Qed.
+
   Lemma bientails_unfold [w] (P Q : Pred w) :
     (P ⊣⊢ₚ Q) <-> forall ι, instprop (wco w) ι -> P ι <-> Q ι.
   Proof. crushPredEntails3. Qed.
@@ -330,13 +335,13 @@ Module Pred
     (P ⊢ₚ Q) <-> forall ι, instprop (wco w) ι -> P ι -> Q ι.
   Proof. crushPredEntails3. Qed.
   Lemma sep_unfold w (P Q : Pred w) :
-    ∀ ι, instprop (wco w) ι -> interface.bi_sep P Q ι ↔ (P ι /\ Q ι).
+    ∀ ι, interface.bi_sep P Q ι ↔ (P ι /\ Q ι).
   Proof. crushPredEntails3. Qed.
   Lemma wand_unfold w (P Q : Pred w) :
-    ∀ ι, instprop (wco w) ι -> interface.bi_wand P Q ι ↔ (P ι → Q ι).
+    ∀ ι, interface.bi_wand P Q ι ↔ (P ι → Q ι).
   Proof. crushPredEntails3. Qed.
   Lemma intuitionistically_unfold w (P : Pred w) :
-    ∀ ι, instprop (wco w) ι -> @derived_connectives.bi_intuitionistically _ P ι <-> P ι.
+    ∀ ι, @derived_connectives.bi_intuitionistically _ P ι <-> P ι.
   Proof. crushPredEntails3. Qed.
 
   Create HintDb punfold.
@@ -450,6 +455,9 @@ Module Pred
     Lemma wand_is_impl [w] (P Q : Pred w) : (P -∗ Q)%I ⊣⊢ₚ (P ->ₚ Q).
     Proof. crushPredEntails3. Qed.
 
+    Lemma sep_is_and [w] (P Q : Pred w) : (P ∗ Q)%I ⊣⊢ₚ (P ∧ Q)%I.
+    Proof. crushPredEntails3. Qed.
+
     Lemma pApply {w} {P Q R : Pred w} : P ⊢ₚ Q -> Q ⊢ₚ R -> P ⊢ₚ R.
     Proof. now transitivity Q. Qed.
 
@@ -479,6 +487,7 @@ Module Pred
 
   Section SubstMod.
     Import ModalNotations.
+    Import ctx.notations.
 
     Lemma acc_pathcond {w1 w2} (ω : w2 ⊒ w1) :
       forall ι,  instprop (wco w1) ι -> instprop (wco w2) (inst (sub_acc ω) ι).
@@ -495,7 +504,7 @@ Module Pred
       fun Rpast ι => forall (ιpast : Valuation w1), inst (sub_acc ω) ιpast = ι -> instprop (wco w1) ιpast -> Rpast ιpast.
     Definition knowing {w1 w2} (ω : w2 ⊒ w1) : Pred w1 -> Pred w2 :=
       fun Rpast ι => (exists (ιpast : Valuation w1), inst (sub_acc ω) ιpast = ι /\ instprop (wco w1) ιpast /\ Rpast ιpast)%type.
-    Definition forgetting {w1 w2} (ω : w2 ⊒ w1) : Pred w2 -> Pred w1 :=
+    Definition forgetting {w1 w2} (ω : w1 ⊒ w2) : Pred w1 -> Pred w2 :=
       fun Rfut ι => Rfut (inst (sub_acc ω) ι).
     Definition unconditionally {w} : (□ Pred) w -> Pred w :=
       fun P => (∀ {w2} (ω : w ⊒ w2), assuming ω (P w2 ω))%I.
@@ -517,8 +526,29 @@ Module Pred
       crushPredEntails3.
     Qed.
 
+    Lemma knowing_sepₚ {w1 w2} {ω : Acc w1 w2} (P1 P2 : Pred w2) :
+      (knowing ω (P1 ∗ P2)) ⊢ knowing ω P1 ∗ knowing ω P2.
+    Proof.
+      unfold knowing.
+      crushPredEntails3.
+    Qed.
+
+    Lemma assuming_sepₚ {w1 w2} {ω : Acc w1 w2} (P1 P2 : Pred w2) :
+      (assuming ω (P1 ∗ P2)) ⊣⊢ assuming ω P1 ∗ assuming ω P2.
+    Proof.
+      unfold assuming.
+      crushPredEntails3.
+    Qed.
+
     #[export] Instance assuming_proper {w1 w2} {ω : Acc w1 w2} :
       Proper (entails ==> entails) (assuming ω).
+    Proof.
+      unfold assuming.
+      crushPredEntails3.
+    Qed.
+
+    #[export] Instance assuming_proper_bientails {w1 w2} {ω : Acc w1 w2} :
+      Proper (bientails ==> bientails) (assuming ω).
     Proof.
       unfold assuming.
       crushPredEntails3.
@@ -635,6 +665,7 @@ Module Pred
       (∀ ι : Valuation w, instprop vt ι <-> a) ->
       ⊢ proprepₚ a vt.
     Proof.
+      unfold proprepₚ.
       crushPredEntails3.
     Qed.
 
@@ -706,9 +737,13 @@ Module Pred
     Lemma forgetting_proprepₚ `{InstPropSubst AT, @SubstLaws AT _} {v w1 w2} {ω : Acc w1 w2}  (t : AT w1) :
       (proprepₚ v (persist t ω) ⊣⊢ forgetting ω (proprepₚ v t))%I.
     Proof.
-      unfold forgetting, proprepₚ.
-      constructor. split;
-      rewrite instprop_persist; auto using acc_pathcond.
+      unfold forgetting, proprepₚ, derived_connectives.bi_wand_iff.
+      constructor.
+      crushPredEntails3.
+      - now apply H4, instprop_persist.
+      - now apply instprop_persist.
+      - now apply H4, instprop_persist.
+      - now apply instprop_persist.
     Qed.
 
     Lemma assuming_refl {w} {P : Pred w} : assuming acc_refl P ⊣⊢ P.
@@ -719,12 +754,58 @@ Module Pred
       - rewrite inst_sub_id in H1; now subst.
     Qed.
 
+    Lemma knowing_refl {w} {P : Pred w} : knowing acc_refl P ⊣⊢ P.
+    Proof.
+      rewrite /knowing.
+      crushPredEntails3.
+      - rewrite inst_sub_id in H0. now subst.
+      - now rewrite inst_sub_id.
+    Qed.
+
+    Lemma knowing_trans {w1 w2 w3} {ω12 : Acc w1 w2} {ω23 : Acc w2 w3} {P : Pred w3} :
+      knowing (acc_trans ω12 ω23) P ⊣⊢ knowing ω12 (knowing ω23 P).
+    Proof.
+      rewrite /knowing.
+      crushPredEntails3.
+      - rewrite sub_acc_trans inst_subst in H0.
+        exists (inst (sub_acc ω23) x).
+        repeat split; try done.
+        { now apply acc_pathcond. }
+        now exists x.
+      - rewrite sub_acc_trans inst_subst.
+        now subst.
+    Qed.
+
+    Lemma assuming_trans {w1 w2 w3} {ω12 : Acc w1 w2} {ω23 : Acc w2 w3} {P : Pred w3} :
+      assuming (acc_trans ω12 ω23) P ⊣⊢ assuming ω12 (assuming ω23 P).
+    Proof.
+      rewrite /assuming.
+      crushPredEntails3.
+      - rewrite sub_acc_trans inst_subst in H0.
+        apply H0; last done.
+        now rewrite H3.
+      - rewrite sub_acc_trans inst_subst in H1.
+        apply (H0 (inst (sub_acc ω23) ιpast)); try done.
+        now apply acc_pathcond.
+    Qed.
+
     Lemma forgetting_refl {w} {P : Pred w} : forgetting acc_refl P ⊣⊢ P.
     Proof.
       rewrite /forgetting.
       crushPredEntails3.
       - now rewrite <-inst_sub_id.
       - now rewrite inst_sub_id.
+    Qed.
+
+    Lemma forgetting_refl' {w} {P : Pred w} (ω : w ⊒ w) :
+      sub_acc ω = sub_id w ->
+      forgetting ω P ⊣⊢ P.
+    Proof.
+      rewrite /forgetting.
+      crushPredEntails3.
+      - rewrite H in H1.
+        now rewrite <-inst_sub_id.
+      - now rewrite H inst_sub_id.
     Qed.
 
     Lemma forgetting_assuming {w1 w2} {ω : Acc w1 w2} {P : Pred w2} :
@@ -851,7 +932,7 @@ Module Pred
     Proof.
       rewrite /forgetting /assuming.
       split; crushPredEntails3.
-      - now subst.
+      - subst; now apply H4.
       - apply (fromEntails _ _ H) with (inst (sub_acc ω) ι);
           auto using acc_pathcond.
     Qed.
@@ -981,6 +1062,38 @@ Module Pred
         now rewrite instprop_subst inst_sub_wk1.
     Qed.
 
+    Lemma knowing_acc_subst_right {w : World} {x σ} `{xIn : (x∷σ ∈ w)%katamaran}
+      {t : Term (w - x∷σ) σ} {P} :
+      (knowing (acc_subst_right t) P : Pred w) ⊣⊢ 
+        (eqₚ (term_var_in xIn) (subst t (sub_shift xIn)) ∗
+           assuming (acc_subst_right t) P)%I.
+    Proof.
+      unfold knowing, assuming.
+      crushPredEntails3.
+      - subst; cbn.
+        rewrite <-inst_lookup, <-inst_subst.
+        now rewrite lookup_sub_single_eq subst_shift_single.
+      - rewrite !inst_sub_single2 in H3 H0.
+        apply (f_equal (fun ι => env.remove (x∷σ) ι xIn)) in H0, H3.
+        rewrite !env.remove_insert in H3, H0.
+        assert (ιpast = x0) by (now transitivity (env.remove (x∷σ) ι xIn)).
+        now subst.
+      - exists (inst (sub_shift xIn) ι).
+        assert (instprop (wco w) (inst (sub_single xIn t) (inst (sub_shift xIn) ι))) as Hpc2.
+        { rewrite inst_sub_single_shift; first done.
+          now rewrite <-inst_subst.
+        }
+        assert (inst t (inst (sub_shift xIn) ι) = env.lookup ι xIn) as Hinst.
+        { now rewrite <-inst_subst. }
+        assert (inst (sub_single xIn t) (inst (sub_shift xIn) ι) = ι) as Hinst2.
+        { now rewrite inst_sub_single_shift. }
+        repeat split; try done.
+        + now rewrite instprop_subst.
+        + apply H1; try done.
+          now rewrite instprop_subst.
+    Qed.
+      
+
     Lemma assuming_acc_snoc_let {w b P v} :
       assuming (@acc_snoc_right w b) P ⊢ assuming (@acc_let_right w b v) P.
     Proof.
@@ -1052,14 +1165,12 @@ Module Pred
       unfold assuming, forgetting, repₚ.
       crushPredEntails3; destruct (env.view ι) as [ι v']; subst; cbn in *.
       - rewrite instprop_subst inst_sub_wk1 in H; subst.
-        constructor.
         crushPredEntails3.
         rewrite inst_sub_wk1.
         apply H0; try done.
         f_equal; try done.
         now apply inst_sub_id.
-      - destruct H0 as [H0].
-        rewrite inst_sub_wk1 in H0.
+      - rewrite inst_sub_wk1 in H0.
         change (env.map _ _) with (inst (sub_id w) ιpast) in H1.
         rewrite inst_sub_id in H1.
         destruct (proj1 (env.inversion_eq_snoc ιpast ι v v') H1) as [-> ->].
@@ -1071,7 +1182,8 @@ Module Pred
     Proof.
       crushPredEntails3.
       - rewrite instprop_snoc in H0.
-        now crushPredEntails3.
+        crushPredEntails3.
+        apply H3; crushPredEntails3.
       - now apply (fromEntails _ _ H).
     Qed.
 
@@ -1079,6 +1191,50 @@ Module Pred
       @bientails (wsnoc w b) (bi_sep (PROP := bi_pred (w := wlet w b v)) P Q)%I (bi_sep (PROP := bi_pred (w := wsnoc w b)) P Q)%I.
     Proof. crushPredEntails3. Qed.
     
+    Lemma forgetting_acc_pathcondition_right_snoc {w : World}
+      {C : PathCondition w} {b : Formula w} 
+      {P : Pred (wpathcondition w (C ▻ b))} :
+      (forgetting (acc_pathcondition_right w (C ▻ b)) P : Pred w) ⊣⊢ 
+        forgetting (acc_pathcondition_right w C) (forgetting (acc_formula_right (w := wpathcondition w C) b) P).
+    Proof.
+      unfold forgetting, acc_pathcondition_right, wpathcondition; cbn.
+      crushPredEntails3.
+      - now rewrite inst_sub_id.
+      - now rewrite inst_sub_id in H0.
+    Qed.
+
+    Lemma assuming_acc_pathcondition_right
+      {w : World} {sc : PathCondition w} {P : Pred w} :
+      (instprop sc : Pred w) ∗ assuming (acc_pathcondition_right w sc) P ⊢ P.
+    Proof.
+      unfold assuming.
+      crushPredEntails3.
+      apply H1.
+      - apply inst_sub_id.
+      - now apply instprop_cat.
+    Qed.
+
+    
+    Lemma forgetting_acc_pathcondition_right_sep {w : World} {P : Pred w} {C : PathCondition w}
+      {Q : Pred (wpathcondition w C)} :
+      (forgetting (acc_pathcondition_right w C) (P ∗ Q) : Pred w) ⊣⊢ 
+        P ∗ forgetting (acc_pathcondition_right w C) Q.
+    Proof.
+      unfold forgetting, acc_pathcondition_right, wpathcondition; cbn.
+      crushPredEntails3.
+      - now rewrite inst_sub_id in H0.
+      - now rewrite inst_sub_id.
+    Qed.
+    
+    Lemma forgetting_acc_pathcondition_right {w : World} {P : Pred w} {C : PathCondition w} :
+      (forgetting (acc_pathcondition_right w C) P : Pred w) ⊣⊢ P.
+    Proof.
+      unfold forgetting, acc_pathcondition_right, wpathcondition; cbn.
+      crushPredEntails3.
+      - now rewrite inst_sub_id in H0.
+      - now rewrite inst_sub_id.
+    Qed.
+      
   End SubstMod.
 
   Module logicalrelation.
@@ -1132,10 +1288,8 @@ Module Pred
         RInst (fun Σ : LCtx => Env (Term Σ) Δ) (Env Val Δ).
     #[export] Instance RUnit : Rel Unit unit := RInst Unit unit.
 
-    #[export] Instance RPathCondition : Rel PathCondition Prop :=
-      MkRel proprepₚ.
-    #[export] Instance RFormula : Rel Formula Prop :=
-      MkRel proprepₚ.
+    #[export] Instance RPathCondition : Rel PathCondition Prop := RInstPropIff PathCondition.
+    #[export] Instance RFormula : Rel Formula Prop := RInstPropIff Formula.
 
     #[export] Instance RChunk : Rel Chunk SCChunk := RInst Chunk SCChunk.
     #[export] Instance RHeap : Rel SHeap SCHeap := RInst SHeap SCHeap.
